WIP use new StringLike

src/Parsers/ContextFreeGrammar.v
@@ -1,22 +1,22 @@
 (** * Definition of Context Free Grammars *)
 Require Import Coq.Strings.String Coq.Lists.List Coq.Program.Program.
 Require Export ADTSynthesis.Parsers.StringLike.
+Require Import ADTSynthesis.Common.
 
 Set Implicit Arguments.
-Local Set Boolean Equality Schemes.
-Local Set Decidable Equality Schemes.
 
-Delimit Scope string_like_scope with string_like.
+Local Open Scope string_like_scope.
+Local Open Scope type_scope.
 
 Section cfg.
-  Variable CharType : Type.
+  Context {string_like} `{HSL : StringLike string_like}.
 
   Section definitions.
     (** An [item] is the basic building block of a context-free
         grammar; it is either a terminal ([CharType]-literal) or a
         nonterminal ([string]). *)
     Inductive item :=
-    | Terminal (_ : CharType)
+    | Terminal (_ : Char)
     | NonTerminal (_ : string).
 
     (** A [productions] is a list of possible [production]s; a
@@ -26,23 +26,22 @@ Section cfg.
     Definition production := list item.
     Definition productions := list production.
 
-    Definition production_dec (CharType_eq_dec : forall x y : CharType, {x = y} + {x <> y})
+    (*Definition production_dec (CharType_eq_dec : forall x y : Char, {x = y} + {x <> y})
                (x y : production) : {x = y} + {x <> y}.
     Proof.
       repeat (apply list_eq_dec; intros);
       decide equality.
       apply string_dec.
-    Defined.
+    Defined.*)
 
-    Definition productions_dec (CharType_eq_dec : forall x y : CharType, {x = y} + {x <> y})
+    (*Definition productions_dec (CharType_eq_dec : forall x y : CharType, {x = y} + {x <> y})
                (x y : productions) : {x = y} + {x <> y}.
     Proof.
       apply list_eq_dec; intros; apply production_dec; assumption.
-    Defined.
+    Defined.*)
 
     (** A [grammar] consists of [productions] to match a string
         against, and a function mapping names to [productions]. *)
-    (** TODO(jgross): look up notations for specifying these nicely *)
     Record grammar :=
       {
         Start_symbol :> string;
@@ -54,61 +53,33 @@ Section cfg.
   End definitions.
 
   Section parse.
-    Variable String : string_like CharType.
     Variable G : grammar.
     (** A parse of a string into [productions] is a [production] in
         that list, together with a list of substrings which cover the
         original string, each of which is a parse of the relevant
         component of the [production]. *)
-    Inductive parse_of : String -> productions -> Type :=
-    | ParseHead : forall str pat pats, parse_of_production str pat
-                                       -> parse_of str (pat::pats)
-    | ParseTail : forall str pat pats, parse_of str pats
-                                       -> parse_of str (pat::pats)
-    with parse_of_production : String -> production -> Type :=
-    | ParseProductionNil : parse_of_production (Empty _) nil
-    | ParseProductionCons : forall str pat strs pats,
-                           parse_of_item str pat
-                           -> parse_of_production strs pats
-                           -> parse_of_production (str ++ strs) (pat::pats)
-    with parse_of_item : String -> item -> Type :=
-    | ParseTerminal : forall x, parse_of_item [[ x ]]%string_like (Terminal x)
-    | ParseNonTerminal : forall nt str, parse_of str (Lookup G nt)
-                                        -> parse_of_item str (NonTerminal nt).
-
-    Definition ParseProductionSingleton str it (p : parse_of_item str it) : parse_of_production str [ it ].
-    Proof.
-      rewrite <- (RightId _ str).
-      constructor; assumption || constructor.
-    Defined.
-
-    Definition ParseProductionApp str1 str2 p1 p2 (pop1 : parse_of_production str1 p1) (pop2 : parse_of_production str2 p2)
-    : parse_of_production (str1 ++ str2) (p1 ++ p2)%list.
-    Proof.
-      induction pop1; simpl.
-      { rewrite LeftId; assumption. }
-      { rewrite Associativity.
-        constructor; assumption. }
-    Defined.
-
-    Definition ParseApp str1 str2 p1 p2 (po1 : parse_of str1 [ p1 ]) (po2 : parse_of str2 [ p2 ])
-    : parse_of (str1 ++ str2) [ (p1 ++ p2)%list ].
-    Proof.
-      inversion_clear po1; inversion_clear po2;
-      try match goal with
-            | [ H : parse_of _ [] |- _ ] => exfalso; revert H; clear; intro H; abstract inversion H
-          end.
-      { constructor. apply ParseProductionApp; assumption. }
-    Defined.
+    Inductive parse_of (str : String) : productions -> Type :=
+    | ParseHead : forall pat pats, parse_of_production str pat
+                                   -> parse_of str (pat::pats)
+    | ParseTail : forall pat pats, parse_of str pats
+                                   -> parse_of str (pat::pats)
+    with parse_of_production (str : String) : production -> Type :=
+    | ParseProductionNil : length str = 0 -> parse_of_production str nil
+    | ParseProductionCons : forall n pat pats,
+                              parse_of_item (take n str) pat
+                              -> parse_of_production (drop n str) pats
+                              -> parse_of_production str (pat::pats)
+    with parse_of_item (str : String) : item -> Type :=
+    | ParseTerminal : forall ch, str ~= [ ch ] -> parse_of_item str (Terminal ch)
+    | ParseNonTerminal : forall nt, parse_of str (Lookup G nt)
+                                    -> parse_of_item str (NonTerminal nt).
   End parse.
 
-  Definition parse_of_grammar (String : string_like CharType) (str : String) (G : grammar) :=
-    parse_of String G str G.
+  Definition parse_of_grammar (str : String) (G : grammar) :=
+    parse_of G str G.
 End cfg.
 
-Arguments parse_of _%type_scope _ _ _%string_like _.
-Arguments parse_of_item _%type_scope _ _ _%string_like _.
-Arguments parse_of_production _%type_scope _ _ _%string_like _.
-Arguments parse_of_grammar _%type_scope _ _%string_like _.
-
-Local Hint Extern 0 => match goal with H : S _ = 0 |- _ => destruct (NPeano.Nat.neq_succ_0 _ H) end.
+Arguments item _ {_}.
+Arguments production _ {_}.
+Arguments productions _ {_}.
+Arguments grammar _ {_}.
