src/Parsers/ContextFreeGrammarProperties.v
@@ -1,41 +1,101 @@
 (** * Properties about Context Free Grammars *)
 Require Import ADTSynthesis.Parsers.StringLike ADTSynthesis.Parsers.ContextFreeGrammar.
 Require Import Coq.Classes.RelationClasses.
+Require Import ADTSynthesis.Common.
 
 Set Implicit Arguments.
 
-Delimit Scope string_like_scope with string_like.
+Local Open Scope list_scope.
 
 Section cfg.
-  Context CharType (String : string_like CharType) (G : grammar CharType).
+  Context {string} `{HSL : StringLike string} `{HSLP : @StringLikeProperties string HSL} (G : grammar string).
+
+  Fixpoint parse_of_respectful (str1 str2 : String) (H : str1 =s str2) (pats : productions string) (p : parse_of G str1 pats) : parse_of G str2 pats
+    := match p in (parse_of _ _ pats) return parse_of G str2 pats with
+         | ParseHead pat pats p' => ParseHead pats (parse_of_production_respectful H p')
+         | ParseTail pat pats p' => ParseTail pat (parse_of_respectful H p')
+       end
+  with parse_of_production_respectful (str1 str2 : String) (H : str1 =s str2) (pat : production string) (p : parse_of_production G str1 pat) : parse_of_production G str2 pat
+       := match p in (parse_of_production _ _ pat) return parse_of_production G str2 pat with
+            | ParseProductionNil pf => ParseProductionNil G str2 (transitivity (eq_sym (length_Proper H)) pf)
+            | ParseProductionCons n pat pats p0 p1 => ParseProductionCons _ n (parse_of_item_respectful (take_Proper eq_refl H) p0) (parse_of_production_respectful (drop_Proper eq_refl H) p1)
+          end
+  with parse_of_item_respectful (str1 str2 : String) (H : str1 =s str2) (it : item string) (p : parse_of_item G str1 it) : parse_of_item G str2 it
+       := match p in (parse_of_item _ _ it) return parse_of_item G str2 it with
+            | ParseTerminal ch pf => ParseTerminal G str2 ch (transitivity (eq_sym (is_char_Proper H eq_refl)) pf)
+            | ParseNonTerminal nt p' => ParseNonTerminal _ (parse_of_respectful H p')
+          end.
+
+  (*Global Instance parse_of_Proper : Proper (beq ==> eq ==> iff) (parse_of G).
+  Proof.
+    split; subst; apply parse_of_respectful; [ assumption | symmetry; assumption ].
+  Qed.
+
+  Global Instance parse_of_production_Proper : Proper (beq ==> eq ==> iff) (parse_of_production G).
+  Proof.
+    split; subst; apply parse_of_production_respectful; [ assumption | symmetry; assumption ].
+  Qed.
+
+  Global Instance parse_of_item_Proper : Proper (beq ==> eq ==> iff) (parse_of_item G).
+  Proof.
+    split; subst; apply parse_of_item_respectful; [ assumption | symmetry; assumption ].
+  Qed.*)
+
+  Definition ParseProductionSingleton str it (p : parse_of_item G str it) : parse_of_production G str [ it ].
+  Proof.
+    econstructor.
+    { eapply parse_of_item_respectful; [ | eassumption ].
+      rewrite take_long; reflexivity. }
+    { constructor.
+      rewrite drop_length; auto with arith. }
+  Defined.
+
+  (*Definition ParseProductionApp str1 str2 p1 p2 (pop1 : parse_of_production str1 p1) (pop2 : parse_of_production str2 p2)
+  : parse_of_production (str1 ++ str2) (p1 ++ p2)%list.
+  Proof.
+    induction pop1; simpl.
+    { rewrite LeftId; assumption. }
+    { rewrite Associativity.
+      constructor; assumption. }
+  Defined.
+
+    Definition ParseApp str1 str2 p1 p2 (po1 : parse_of str1 [ p1 ]) (po2 : parse_of str2 [ p2 ])
+    : parse_of (str1 ++ str2) [ (p1 ++ p2)%list ].
+    Proof.
+      inversion_clear po1; inversion_clear po2;
+      try match goal with
+            | [ H : parse_of _ [] |- _ ] => exfalso; revert H; clear; intro H; abstract inversion H
+          end.
+      { constructor. apply ParseProductionApp; assumption. }
+    Defined.*)
 
   Section definitions.
     Context (P : String -> String.string -> Type).
 
     Definition Forall_parse_of_item'
-               (Forall_parse_of : forall {str pats} (p : parse_of String G str pats), Type)
-               {str it} (p : parse_of_item String G str it)
+               (Forall_parse_of : forall {str pats} (p : parse_of G str pats), Type)
+               {str it} (p : parse_of_item G str it)
       := match p return Type with
-           | ParseTerminal x => unit
-           | ParseNonTerminal name str p'
-             => (P str name * Forall_parse_of p')%type
+           | ParseTerminal ch pf => unit
+           | ParseNonTerminal nt p'
+             => (P str nt * Forall_parse_of p')%type
          end.
 
-    Fixpoint Forall_parse_of {str pats} (p : parse_of String G str pats)
+    Fixpoint Forall_parse_of {str pats} (p : parse_of G str pats)
       := match p with
-           | ParseHead str pat pats p'
+           | ParseHead pat pats p'
              => Forall_parse_of_production p'
-           | ParseTail _ _ _ p'
+           | ParseTail _ _ p'
              => Forall_parse_of p'
          end
-    with Forall_parse_of_production {str pat} (p : parse_of_production String G str pat)
+    with Forall_parse_of_production {str pat} (p : parse_of_production G str pat)
          := match p return Type with
-              | ParseProductionNil => unit
-              | ParseProductionCons str pat strs pats p' p''
+              | ParseProductionNil pf => unit
+              | ParseProductionCons pat strs pats p' p''
                 => (Forall_parse_of_item' (@Forall_parse_of) p' * Forall_parse_of_production p'')%type
             end.
 
-    Definition Forall_parse_of_item {str it} (p : parse_of_item String G str it)
+    Definition Forall_parse_of_item {str it} (p : parse_of_item G str it)
       := @Forall_parse_of_item' (@Forall_parse_of) str it p.
   End definitions.
 
@@ -44,7 +104,7 @@ Section cfg.
 
     Definition expand_forall_parse_of_item'
                {str}
-               {Forall_parse_of : forall P {str pats} (p : parse_of String G str pats), Type}
+               {Forall_parse_of : forall P {str pats} (p : parse_of G str pats), Type}
                (expand : forall {pats p}, @Forall_parse_of P str pats p -> @Forall_parse_of P' str pats p)
                (f : forall n, P str n -> P' str n)
                {it p}
@@ -62,51 +122,51 @@ Section cfg.
     Fixpoint expand_forall_parse_of
              str
              (f : forall str', str' ≤s str -> forall n, P str' n -> P' str' n)
-             pats (p : parse_of String G str pats)
+             pats (p : parse_of G str pats)
              {struct p}
     : Forall_parse_of P p -> Forall_parse_of P' p
     with expand_forall_parse_of_production
            str
            (f : forall str', str' ≤s str -> forall n, P str' n -> P' str' n)
-           pat (p : parse_of_production String G str pat)
+           pat (p : parse_of_production G str pat)
            {struct p}
          : Forall_parse_of_production P p -> Forall_parse_of_production P' p.
     Proof.
-      { exact (match p in parse_of _ _ str' pats'
-                     return (forall str'', str'' ≤s str' -> forall n, P str'' n -> P' str'' n)
+      { exact (match p in parse_of _ _ pats'
+                     return (forall str'', str'' ≤s str -> forall n, P str'' n -> P' str'' n)
                             -> Forall_parse_of P p -> Forall_parse_of P' p
                with
-                 | ParseHead _ _ _ p'
+                 | ParseHead _ _ p'
                    => fun f' => @expand_forall_parse_of_production _ f' _ p'
-                 | ParseTail _ _ _ p'
+                 | ParseTail _ _ p'
                    => fun f' => @expand_forall_parse_of _ f' _ p'
                end f). }
-      { refine (match p in parse_of_production _ _ str' pats'
-                      return (forall str'', str'' ≤s str' -> forall n, P str'' n -> P' str'' n)
+      { refine (match p in parse_of_production _ _ pats'
+                      return (forall str'', str'' ≤s str -> forall n, P str'' n -> P' str'' n)
                              -> Forall_parse_of_production P p -> Forall_parse_of_production P' p
                 with
-                  | ParseProductionNil => fun _ x => x
-                  | ParseProductionCons str' pat strs' pats p' p''
+                  | ParseProductionNil pf => fun _ x => x
+                  | ParseProductionCons pat strs' pats p' p''
                     => fun f' ab
                        => (_ : Forall_parse_of_item' _ (@Forall_parse_of _) _,
                            expand_forall_parse_of_production
                              _
-                             (fun str'' pf'' => f' str'' (transitivity pf'' (str_le2_append _ _)))
+                             (fun str'' pf'' => f' str'' (transitivity pf'' str_le_drop))
                              _ _
                              (snd ab))
                 end f).
         destruct p'; simpl.
         { exact tt. }
-        { refine (f' _ (str_le1_append _ _) _ (fst (fst ab)),
+        { refine (f' _ str_le_take _ (fst (fst ab)),
                   expand_forall_parse_of _ _ _ _ (snd (fst ab))).
           intros ??; apply f'.
-          etransitivity; [ eassumption | exact (str_le1_append _ _) ]. } }
+          etransitivity; [ eassumption | exact str_le_take ]. } }
     Defined.
 
     Global Arguments expand_forall_parse_of : simpl never.
     Global Arguments expand_forall_parse_of_production : simpl never.
 
-    Definition expand_forall_parse_of_item {str} f {it} {p : parse_of_item String G str it}
+    Definition expand_forall_parse_of_item {str} f {it} {p : parse_of_item G str it}
       := @expand_forall_parse_of_item' str _ (@expand_forall_parse_of str f) (f _ (reflexivity _)) it p.
 
     Global Arguments expand_forall_parse_of_item : simpl never.
