src/Parsers/Grammars/ABStar.v
@@ -7,52 +7,51 @@ Set Implicit Arguments.
 Section ab_star.
   Local Open Scope string_scope.
 
-  Definition ab_star_grammar : grammar Ascii.ascii :=
+  Definition ab_star_grammar : grammar string :=
     {| Start_symbol := "(ab)*";
        Lookup := [[[ ("(ab)*" ::== << nil
                                      | $< "a"%char $ "b"%char $ "(ab)*" >$ >> ) ]]]%prods_assignment;
        Valid_nonterminals := ("(ab)*"::nil)%string |}.
 
-  Definition ab_star_grammar' : grammar Ascii.ascii :=
+  Definition ab_star_grammar' : grammar string :=
     {| Start_symbol := "(ab)*";
-       Lookup := fun _ => nil::(Terminal "a"%char::Terminal "b"%char::NonTerminal _ "(ab)*"%string::nil)::nil;
+       Lookup := fun _ => nil::(Terminal "a"%char::Terminal "b"%char::NonTerminal "(ab)*"%string::nil)::nil;
        Valid_nonterminals := ("(ab)*"::nil)%string |}.
 End ab_star.
 
 Create HintDb cfg discriminated.
 Hint Constructors parse_of parse_of_production parse_of_item : cfg.
-Hint Resolve ParseProductionSingleton ParseProductionApp ParseApp : cfg.
 
 Section tests.
-  Example ab_star_parses_empty : parse_of_grammar string_stringlike (Empty _) ab_star_grammar.
+  Example ab_star_parses_empty : parse_of_grammar ""%string ab_star_grammar.
   Proof.
     hnf; simpl.
     repeat constructor.
   Defined.
 
-  Example ab_star_parses_ab : parse_of_grammar string_stringlike "ab"%string ab_star_grammar.
+  Example ab_star_parses_ab : parse_of_grammar "ab"%string ab_star_grammar.
   Proof.
     hnf; simpl.
-    constructor (constructor); simpl.
-    apply ParseProductionCons with (str := "a"%string) (strs := "b"%string).
-    { refine (ParseTerminal _ _ _). }
-    { apply ParseProductionCons with (str := "b"%string) (strs := ""%string).
-      { refine (ParseTerminal _ _ _). }
-      { apply ParseProductionCons with (str := ""%string) (strs := ""%string);
+    apply ParseTail, ParseHead.
+    apply ParseProductionCons with (n := 1); simpl.
+    { refine (ParseTerminal _ _ _ _); reflexivity. }
+    { apply ParseProductionCons with (n := 1); simpl.
+      { refine (ParseTerminal _ _ _ _); reflexivity. }
+      { apply ParseProductionCons with (n := 1); simpl;
         repeat (simpl; constructor). } }
   Defined.
 
-  Example ab_star_parses_abab : parse_of_grammar string_stringlike "abab"%string ab_star_grammar.
+  Example ab_star_parses_abab : parse_of_grammar "abab"%string ab_star_grammar.
   Proof.
     hnf; simpl.
-    constructor (constructor); simpl.
-    apply ParseProductionCons with (str := "a"%string) (strs := "bab"%string).
-    { refine (ParseTerminal _ _ _). }
-    { apply ParseProductionCons with (str := "b"%string) (strs := "ab"%string).
-      { refine (ParseTerminal _ _ _). }
-      { apply ParseProductionCons with (str := "ab"%string) (strs := ""%string).
-        { constructor.
-          apply ab_star_parses_ab. }
-        { constructor. } } }
+    apply ParseTail, ParseHead.
+    apply ParseProductionCons with (n := 1); simpl.
+    { refine (ParseTerminal _ _ _ _); reflexivity. }
+    { apply ParseProductionCons with (n := 1); simpl.
+      { refine (ParseTerminal _ _ _ _); reflexivity. }
+      { apply ParseProductionCons with (n := 2); simpl;
+        try solve [ repeat (simpl; constructor) ].
+        constructor.
+        apply ab_star_parses_ab. } }
   Defined.
 End tests.
