src/Parsers/Grammars/ExpressionNumPlus.v
@@ -8,7 +8,7 @@ Section num_plus.
   Local Open Scope string_scope.
   Local Open Scope grammar_scope.
 
-  Definition plus_expr_grammar : grammar Ascii.ascii :=
+  Definition plus_expr_grammar : grammar string :=
     [[[ ("expr" ::== << $< "number" >$
                       | $< "number" $ #"+" $ "expr" >$ >>);;
         ("digit" ::== << $< #"0" >$ | $< #"1" >$ | $< #"2" >$ | $< #"3" >$ | $< #"4" >$ | $< #"5" >$ | $< #"6" >$ | $< #"7" >$ | $< #"8" >$ | $< #"9" >$ >>);;
@@ -20,22 +20,31 @@ Section tests.
   Local Arguments append : simpl never.
 
   Local Ltac fin :=
-    repeat first [ apply ParseProductionSingleton
-                 | apply ParseProductionCons
+    repeat first [ idtac;
+                   (lazymatch goal with
+                   | [ |- parse_of_production _ ?s (Terminal _ :: _) ]
+                     => apply ParseProductionCons with (n := 1)
+                   | [ |- parse_of_production _ ?s (_ :: nil) ]
+                     => apply ParseProductionCons with (n := length s)
+                   | [ |- parse_of_production _ ?s (_ :: Terminal _ :: nil) ]
+                     => apply ParseProductionCons with (n := length s - 1)
+                   | _ => apply ParseProductionCons with (n := 1); solve [ fin ]
+                    end)
                  | apply ParseProductionNil
                  | refine (ParseTerminal _ _ _)
                  | refine (ParseNonTerminal _ _)
                  | progress simpl
                  | solve [ constructor (solve [ fin ]) ] ].
 
-  Example plus_expr_parses_1 : parse_of_grammar string_stringlike "1+2+3+4+5"%string plus_expr_grammar.
+  Example plus_expr_parses_1 : parse_of_grammar "1+2+3+4+5"%string plus_expr_grammar.
   Proof.
     hnf; simpl.
     apply ParseTail, ParseHead.
     match goal with
-      | [ |- parse_of_production _ _ ?s _ ] => set (n := s)
+      | [ |- parse_of_production _ ?s _ ] => set (n := s)
     end.
     change n with ("1" ++ ("+" ++ ("2" ++ ("+" ++ ("3" ++ ("+" ++ ("4" ++ ("+" ++ "5"))))))))%string; subst n.
+    simpl.
     fin.
   Defined.
 End tests.
