src/Parsers/Grammars/ExpressionNumPlusParen.v
@@ -8,7 +8,7 @@ Section num_plus_paren.
   Local Open Scope string_scope.
   Local Open Scope grammar_scope.
 
-  Definition plus_expr_grammar : grammar Ascii.ascii :=
+  Definition plus_expr_grammar : grammar string :=
     [[[ ("expr" ::== << $< "pexpr" >$
                       | $< "pexpr" $ #"+" $ "expr" >$ >>);;
         ("pexpr" ::== << $< "number" >$
@@ -22,22 +22,46 @@ Section tests.
   Local Arguments append : simpl never.
 
   Local Ltac fin :=
-    repeat first [ apply ParseProductionSingleton
-                 | apply ParseProductionCons
+    repeat first [ idtac;
+                   (lazymatch goal with
+                   | [ |- parse_of_production _ ?s (Terminal _ :: _) ]
+                     => apply ParseProductionCons with (n := 1)
+                   | [ |- parse_of_production _ ?s (_ :: nil) ]
+                     => apply ParseProductionCons with (n := length s)
+                   | [ |- parse_of_production _ ?s (_ :: Terminal _ :: nil) ]
+                     => apply ParseProductionCons with (n := length s - 1)
+                    end)
                  | apply ParseProductionNil
                  | refine (ParseTerminal _ _ _)
                  | refine (ParseNonTerminal _ _)
                  | progress simpl
                  | solve [ constructor (solve [ fin ]) ] ].
 
-  Example plus_expr_parses_1 : parse_of_grammar string_stringlike "1+(2+3)+4+5"%string plus_expr_grammar.
+  Example plus_expr_parses_1 : parse_of_grammar "1+(2+3)+4+5"%string plus_expr_grammar.
   Proof.
     hnf; simpl.
     apply ParseTail, ParseHead.
     match goal with
-      | [ |- parse_of_production _ _ ?s _ ] => set (n := s)
+      | [ |- parse_of_production _ ?s _ ] => set (n := s)
     end.
     change n with (((("1"))) ++ ("+" ++ (("(" ++ ((((("2"))) ++ ("+" ++ ("3"))) ++ ")")) ++ ("+" ++ ("4" ++ ("+" ++ "5"))))))%string; subst n.
-    fin.
+    apply ParseProductionCons with (n := 1); [ solve [ fin ] | simpl ].
+    apply ParseProductionCons with (n := 1); [ solve [ fin ] | simpl ].
+    apply ParseProductionCons with (n := 9); [ | solve [ fin ] ].
+    constructor; simpl.
+    apply ParseTail, ParseHead.
+    apply ParseProductionCons with (n := 5); simpl.
+    { constructor; simpl.
+      apply ParseTail, ParseHead.
+      apply ParseProductionCons with (n := 1); [ solve [ fin ] | simpl ].
+      apply ParseProductionCons with (n := 3); simpl; [ | solve [ fin ] ].
+      constructor; simpl.
+      apply ParseTail, ParseHead; fin.
+      apply ParseProductionCons with (n := 1); fin. }
+    { apply ParseProductionCons with (n := 1); simpl; [ solve [ fin ] | ].
+      apply ParseProductionCons with (n := 3); simpl; [ | solve [ fin ] ].
+      constructor; simpl.
+      apply ParseTail, ParseHead; fin.
+      apply ParseProductionCons with (n := 1); fin. }
   Defined.
 End tests.
