src/Parsers/Grammars/Trivial.v
@@ -5,28 +5,29 @@ Require Import ADTSynthesis.Parsers.ContextFreeGrammar.
 Set Implicit Arguments.
 
 Section generic.
-  Variable CharType : Type.
-  Variable String : string_like CharType.
+  Context {string} {HSL : StringLike string}.
 
-  Definition trivial_grammar : grammar CharType :=
+  Definition trivial_grammar : grammar string :=
     {| Start_symbol := "";
        Lookup := fun _ => nil::nil;
        Valid_nonterminals := ""%string::nil |}.
 
-  Definition trivial_grammar_parses_empty_string : parse_of_grammar _ (Empty String) trivial_grammar.
+  Definition trivial_grammar_parses_empty_string {s} (H : length s = 0)
+  : parse_of_grammar s trivial_grammar.
   Proof.
     hnf; simpl.
     apply ParseHead.
-    constructor.
+    constructor; assumption.
   Defined.
 
-  Lemma trivial_grammar_parses_only_empty_string s : parse_of_grammar _ s trivial_grammar -> s = Empty String.
+  Lemma trivial_grammar_parses_only_empty_string s : parse_of_grammar s trivial_grammar -> length s = 0.
   Proof.
     intro H; hnf in H; simpl in H.
     repeat match goal with
              | _ => reflexivity
-             | [ H : parse_of _ _ _ _ |- _ ] => inversion_clear H
-             | [ H : parse_of_production _ _ _ _ |- _ ] => inversion_clear H
+             | _ => assumption
+             | [ H : parse_of _ _ _ |- _ ] => inversion_clear H
+             | [ H : parse_of_production _ _ _ |- _ ] => inversion_clear H
            end.
   Qed.
 End generic.
