src/Parsers/BooleanBaseTypes.v
@@ -4,56 +4,36 @@ Require Import ADTSynthesis.Parsers.BaseTypes ADTSynthesis.Parsers.ContextFreeGr
 Require Import ADTSynthesis.Parsers.MinimalParse.
 Require Import ADTSynthesis.Common.
 
-Local Coercion is_true : bool >-> Sortclass.
-
 Local Open Scope string_like_scope.
 
 Section general.
-  Context {CharType} {String : string_like CharType} {G : grammar CharType}.
+  Context {string} {HSL : StringLike string} {G : grammar string}.
 
   Class boolean_parser_dataT :=
     { predata :> parser_computational_predataT;
-      split_stateT : String -> Type;
-      data' :> _ := {| BaseTypes.predata := predata ; BaseTypes.split_stateT := fun _ _ _ => split_stateT |};
       split_string_for_production
-      : forall it its,
-          StringWithSplitState String split_stateT
-          -> list (StringWithSplitState String split_stateT * StringWithSplitState String split_stateT);
-      split_string_for_production_correct
-      : forall it its (str : StringWithSplitState String split_stateT),
-          let P f := List.Forall f (split_string_for_production it its str) in
-          P (fun s1s2 =>
-               (fst s1s2 ++ snd s1s2 =s str) = true);
-      premethods :> parser_computational_dataT'
-      := @Build_parser_computational_dataT'
-           _ String data'
-           (fun _ _ => split_string_for_production)
-           (fun _ _ => split_string_for_production_correct) }.
+      : item string -> production string -> String -> list nat }.
 
-  Definition split_list_completeT `{data : @parser_computational_types_dataT _ String}
+  Global Coercion predata : boolean_parser_dataT >-> parser_computational_predataT.
+
+  Definition split_list_completeT `{data : @parser_computational_predataT}
              {str0 valid}
-             (it : item CharType) (its : production CharType)
-             (str : StringWithSplitState String (@BaseTypes.split_stateT _ _ data str0 valid (it::its : production CharType)))
+             (it : item string) (its : production string)
+             (str : String)
              (pf : str ≤s str0)
-             (split_list : list (StringWithSplitState String (@BaseTypes.split_stateT _ _ data str0 valid it)
-                                 * StringWithSplitState String (@BaseTypes.split_stateT _ _ data str0 valid its)))
+             (split_list : list nat)
 
-    := ({ s1s2 : String * String
-                 & (fst s1s2 ++ snd s1s2 =s str)
-                   * (minimal_parse_of_item (G := G) (predata := @BaseTypes.predata _ _ data) str0 valid (fst s1s2) it)
-                   * (minimal_parse_of_production (G := G) str0 valid (snd s1s2) its) }%type)
-       -> ({ s1s2 : _
-                    & (In s1s2 split_list)
-                      * (minimal_parse_of_item (G := G) str0 valid (fst s1s2) it)
-                      * (minimal_parse_of_production (G := G) str0 valid (snd s1s2) its) }%type).
-
-  Coercion parser_computational_types_dataT__of__boolean_parser_dataT {data : boolean_parser_dataT}
-  : @parser_computational_types_dataT _ String
-    := {| BaseTypes.predata := predata ; BaseTypes.split_stateT := fun _ _ _ => split_stateT |}.
+    := ({ n : nat
+              & (minimal_parse_of_item (G := G) (predata := data) str0 valid (take n str) it)
+                * (minimal_parse_of_production (G := G) str0 valid (drop n str) its) }%type)
+       -> ({ n : nat
+                 & (In n split_list)
+                   * (minimal_parse_of_item (G := G) str0 valid (take n str) it)
+                   * (minimal_parse_of_production (G := G) str0 valid (drop n str) its) }%type).
 
   Class boolean_parser_completeness_dataT' `{data : boolean_parser_dataT} :=
     { split_string_for_production_complete
-      : forall str0 valid (str : StringWithSplitState String split_stateT) (pf : str ≤s str0) nt,
+      : forall str0 valid str (pf : str ≤s str0) nt,
           is_valid_nonterminal initial_nonterminals_data nt
           -> ForallT
                (Forall_tails
