src/Parsers/ContextFreeGrammarNotations.v
@@ -1,7 +1,8 @@
 Require Import Coq.Strings.String Coq.Strings.Ascii Coq.Lists.List.
 Require Import ADTSynthesis.Parsers.ContextFreeGrammar.
+Require Import ADTSynthesis.Parsers.StringLike.Examples.
 
-Fixpoint production_of_string (s : string) : production Ascii.ascii
+Fixpoint production_of_string (s : string) : production string
   := match s with
        | EmptyString => nil
        | String.String ch s' => (Terminal ch)::production_of_string s'
@@ -17,15 +18,15 @@ Fixpoint list_to_productions {T} (default : T) (ls : list (string * T)) : string
                                    else list_to_productions default ls' s
      end.
 
-Fixpoint list_to_grammar {T} (default : productions T) (ls : list (string * productions T)) : grammar T
+Fixpoint list_to_grammar {T} `{StringLike T} (default : productions T) (ls : list (string * productions T)) : grammar T
   := {| Start_symbol := hd ""%string (map fst ls);
         Lookup := list_to_productions default ls;
         Valid_nonterminals := map fst ls |}.
 
-Definition item_ascii := item Ascii.ascii.
+Definition item_ascii := item string.
 Coercion item_of_char (ch : Ascii.ascii) : item_ascii := Terminal ch.
-Coercion item_of_string (nt : string) : item_ascii := NonTerminal _ nt.
-Definition item_ascii_cons : item_ascii -> production Ascii.ascii -> production Ascii.ascii := cons.
+Coercion item_of_string (nt : string) : item_ascii := NonTerminal nt.
+Definition item_ascii_cons : item_ascii -> production string -> production string := cons.
 Global Arguments item_ascii_cons / .
 Global Arguments item_of_char / .
 Global Arguments item_of_string / .
