src/Parsers/WellFoundedParse.v
@@ -3,40 +3,39 @@ Require Import Coq.Strings.String Coq.Lists.List Coq.Program.Program Coq.Program
 Require Import ADTSynthesis.Parsers.ContextFreeGrammar.
 
 Section rel.
-  Context {CharType} {String : string_like CharType} {G : grammar CharType}.
+  Context {string} {HSL : StringLike string} {G : grammar string}.
 
   Section size.
-
     Definition size_of_parse_item'
-               (size_of_parse : forall {str pats} (p : parse_of String G str pats), nat)
-               {str it} (p : parse_of_item String G str it) : nat
+               (size_of_parse : forall {str pats} (p : parse_of G str pats), nat)
+               {str it} (p : parse_of_item G str it) : nat
       := match p with
-           | ParseTerminal _ => 0
-           | ParseNonTerminal _ _ p' => S (size_of_parse p')
+           | ParseTerminal _ _ => 0
+           | ParseNonTerminal _ p' => S (size_of_parse p')
          end.
 
-    Fixpoint size_of_parse {str pats} (p : parse_of String G str pats) : nat
+    Fixpoint size_of_parse {str pats} (p : parse_of G str pats) : nat
       := match p with
-           | ParseHead _ _ _ p' => S (size_of_parse_production p')
-           | ParseTail _ _ _ p' => S (size_of_parse p')
+           | ParseHead _ _ p' => S (size_of_parse_production p')
+           | ParseTail _ _ p' => S (size_of_parse p')
          end
-    with size_of_parse_production {str pat} (p : parse_of_production String G str pat) : nat
+    with size_of_parse_production {str pat} (p : parse_of_production G str pat) : nat
          := match p with
-              | ParseProductionNil => 0
-              | ParseProductionCons _ _ _ _ p' p''
+              | ParseProductionNil _ => 0
+              | ParseProductionCons _ _ _ p' p''
                 => S (size_of_parse_item' (@size_of_parse) p' + size_of_parse_production p'')
             end.
 
     Definition size_of_parse_item
-               {str it} (p : parse_of_item String G str it) : nat
+               {str it} (p : parse_of_item G str it) : nat
       := @size_of_parse_item' (@size_of_parse) str it p.
   End size.
 
-  Definition parse_of_lt {str pats} : relation (parse_of String G str pats)
+  Definition parse_of_lt {str pats} : relation (parse_of G str pats)
     := ltof _ size_of_parse.
-  Definition parse_of_production_lt {str pat} : relation (parse_of_production String G str pat)
+  Definition parse_of_production_lt {str pat} : relation (parse_of_production G str pat)
     := ltof _ size_of_parse_production.
-  Definition parse_of_item_lt {str it} : relation (parse_of_item String G str it)
+  Definition parse_of_item_lt {str it} : relation (parse_of_item G str it)
     := ltof _ size_of_parse_item.
 
   Definition parse_of_wf {str pats} : well_founded (@parse_of_lt str pats)
